src/mem/Thread.v
@@ -30,18 +30,19 @@ End Thread.
 Module Threads.
   Definition t := Ident.Map.t Thread.t.
 
+  Definition empty := Ident.Map.empty Thread.t.
+
   Inductive is_terminal (p:t): Prop :=
   | is_terminal_intro
       (TERMINAL:
-         forall i th
-           (S: Ident.Map.find i p = Some th),
+         forall i th (THREAD: Ident.Map.find i p = Some th),
            Thread.is_terminal th)
   .
 
   Inductive step: forall (p1:t) (i:Ident.t) (e:option ThreadEvent.t) (p1:t), Prop :=
   | step_intro
-      p1 i th1 e th2
-      (TH1: Ident.Map.find i p1 = Some th1)
+      p1 th1 th2 i e
+      (THREAD: Ident.Map.find i p1 = Some th1)
       (STEP: Thread.step th1 e th2):
       step p1 i e (Ident.Map.add i th2 p1)
   .
